 Links: [[01 Reflection of Light]], [[02 Object and Image]], [[03 Spherical Mirror]]
___
# Magnification for Spherical Mirror
## Lateral Magnification 
aka Transverse Magnification

![[Lateral Magnification.png]]
(only applies when object is $\perp$ to principal axis)

- Object is placed $\perp$ to PA
- Farther the image, the larger it is.
- If object and image are one the same side of the mirror, image will be inverted.
	- Real image will have real image.
	- Real img & obj $\to$ erect
	- Virtual img & obj $\to$ erect
- If object and image are on the opposite sides, the image is erect.
	- Real image will have virtual image.
	- Real img & virtual obj $\to$ erect
	- Virtual img & real obj $\to$ erect


### Lateral Magnification Formula
![[Lateral Magnification Formula.png]]


> $$\begin{split}
> m &= \frac{h_{i}}{h_{o}} = \frac{-A'B'}{AB} \\
> \\
> 
> \bigtriangleup \text{APB} &\sim \bigtriangleup \text{A'PB'} \\
> \\
> 
> \frac{AB}{AP} &= \frac{A'B'}{A'P} \\
> \frac{A'P}{AP} &= \frac{A'B'}{AB} \\
> \frac{-v}{-u} &=  \frac{v}{u} \\
> \end{split}$$
Thus,
>$$m = \frac{h_{i}}{h_{o}} = \frac{y_{i}}{y_{o}} =  \frac{-v}{u}$$


- The farther away the image is the greater $m$ is. ($m \propto v$)
- If $v\ \&\ u$ have the same sign $m$ is $-ve$, i.e. inverted.
- If $v\ \&\ u$ have the opposite sign $m$ is $+ve$, i.e. erect.

Putting the value of v,
> $$
> \begin{split}
> v &= \frac{uf}{u-f} \\
> m &= \frac{-\frac{uf}{u-f}}{u} \\
> m &= \frac{-uf}{(u-f)(u)} \\
> m &= \frac{-f}{u-f} \\
> m &= \frac{f}{f-u}
> \end{split}
> $$


## Longitudinal Magnification

When the object is placed along the principal axis. 

### When object is not very small

![[Longitudional Magnification.png]]

> $$m_{l} = \frac{l_{i}}{l_{o}} = -\frac{|u_{B}-u_{A}|}{|v_{B}-v_{A}|}$$

### When object is very small
![[Long Mag if obj small.png]]

> $$m_{l} = \frac{l_{i}}{l_{o}} = \frac{dv}{du}$$

We know that, 

> $$v^{-1} + u^{-1} = f^{-1}$$

Differentiating the whole equation independently, 

> $$\frac{-1}{v^{2}} dv - \frac{1}{u^{2}}du = 0$$
> $$\implies dv = \frac{-v^{2}}{u^{2}}du$$
> $$\implies m_{l} = \frac{dv}{du} = \frac{-v^{2}}{u^{2}}$$

Thus, 
> $$m_{l} = \frac{-v^{2}}{u^{2}}$$

Or, using transverse magnification,

> $$m_{l} = -m_{t}^{2} = - \frac{ v^{2} }{ u^{2} }$$
> $$\text{or, }\ m_{l} = -\left( \frac{f}{f-u} \right)^{2}$$
> 
> where, $$m_{t} = \frac{-v}{u}$$


