Links: [[15 Thin Lens]] 
___
# Magnification for Lens
## Transverse Magnification
When object is placed perpendicular to PA.
Similar to [[06 Magnification#Lateral Magnification]] in mirror. 

![[Pasted image 20230518193253.png]]

- The farther the image, the larger it is. 
- If both object and image are on the same side then image is erect. 
	- Real object has erect virtual image
	- Virtual object has erect virtual image
- If both object and image are on opposite sides then image is inverted. 
	- Real object has inverted real image
	- Virtual object has inverted virtual image

### Lateral Magnification Formula 

![[Pasted image 20230518193753.png]]

> $$
> \begin{split}
> \triangle ABP \sim \triangle A'B'P,& \\
> \frac{ AB }{ AP } &= \frac{ A'B' }{ A'P } \\
> \frac{ A'P }{ AP } &= \frac{ A'B' }{ AB } \\
> \frac{ h_{i} }{ h_{o} } &= \frac{ -A'B' }{ AB } \\
> \\
> m &= \frac{ -(v) }{ -u } \\
> m &= \frac{v}{u}
> \end{split}
> $$

Thus,
$$m = \frac{ h_{i} }{ h_{o} } = \frac{ v }{ u }$$

Using formula for v, similar to mirror,
$$m = \frac{ f }{ u + f }$$

If u and v have the same sign, magnification is +ve and image is erect. 
If u and v have the opposite signs, magnification is -ve and image is inverted. 

Thus to see an inverted, erect and enlarged image we need convex lens and the object distance should be less than the focal length. 

If object is at 2f, then image is at the other 2f but inverted of the same size. The minimum separation between a real object and a real image is 4f, when both of them are at 2f. 

## Longitudinal Magnification
When the object is placed parallel to the principal axis. 
Similar to [[06 Magnification#Longitudinal Magnification]] in mirror.
When object is not very small, 
$$m_{l} = \left| \frac{ u_{B} - u_{A} }{ v_{B} - v_{A} } \right|$$

If object is very small,
$$
\begin{split}
v^{-1} - u^{-1} &= f^{-1} \\
\text{ Differentiating the equation,} &\\
\frac{ -1 }{ v^{2} } dv + \frac{ 1 }{ u^{2} }du &= 0 \\
\frac{ 1 }{ v^{2} }dv &= \frac{ 1 }{ u^{2} }du \\
\frac{ dv }{ du } &= \frac{ v^{2} }{ u^{2} }
\end{split}
$$

Thus,
$$m_{l} = \frac{ v^{2} }{ u^{2} } = m_{t}^{2} = \left( \frac{ f }{ f+u } \right)^{2}$$
