Links:  
___
# Trigonometric Substitution
If there is square root, we try to remove it by using trigonometric substitution. 

$$
\begin{split}
\sqrt{ a^{2} - x^{2} } &\ce{ -> } x = a\cos \theta \text{ or } x = a\sin \theta 
\\
\sqrt{ x^{2} - a^{2} } &\ce{ -> } x = a\sec \theta \text{ or } x = a\csc \theta 
\\
\sqrt{ x^{2} + a^{2} } &\ce{ -> } x = a\tan \theta \text{ or } x = a\cot \theta 
\\
\sqrt{ \frac{ a-x }{ a+x } } &\ce{ -> } x = a\cos 2\theta  
\\
\sqrt{ a + x } + \sqrt{ a - x } &\ce{ -> } x = a\cos 2\theta 
\end{split}
$$

Some other substitutions,
$$
\begin{split}
\sqrt{ (x-a)(x-b) } &\ce{ -> } x = a\sec^{2}\theta - b\tan ^{2} \theta \\
\sqrt{ (x-a)(b-x) } &\ce{ -> } x = a\sin^{2}\theta - b\cos ^{2} \theta \\
\end{split}
$$

To convert back to x, use the triangle and put the values of the corresponding trig ratio from there. 

#### Examples
![[Pasted image 20230928180828.png]]

We can also use substitution to remove inverse trig functions,
![[Pasted image 20230928181355.png]]

![[Pasted image 20230928184651.png]]
![[Pasted image 20230928184708.png]]