Links: [[00 Quadratic Equations and Expressions]]
___
# Roots of a Quadratic
if $a,b,c$ are constants and $ax^{2}+bx+c=0$, then
> $$\begin{split}
a(x-\alpha)(x-\beta) & = 0\\
\implies  x = \alpha &\text{ or } x = \beta
\end{split}$$

Every quadratic equation has exactly two roots. 
> $$x = \frac{-b \pm \sqrt{b^{2} - 4ac}}{2a}$$

In saying solution, we only count unique values. In saying roots, we count all values.
- The solution of that quadratic is $x=1$. The roots of the quadratic are $x=1$ and $x=1$.

$ax^{2} + bx + c \equiv a(x-\alpha)(x-\beta)$ is an identity,  

> $ax^{2} + bx + c \equiv a(x-\alpha)(x-\beta)$
  $\implies ax^{2} + bx + c \equiv ax^{2} - a(\alpha+\beta) + a \cdot \alpha \beta$
  $\implies b = -a(\alpha+\beta) \text{ and } c = a \cdot \alpha \beta$


From the previous result,
   - Sum of roots, $S$
>  	$$\alpha + \beta = \frac{b}{a}$$
	- Product of the roots, $P$
> $$\alpha \beta = \frac{c}{a}$$

> Hence, $ax^{2} + bx + c = 0$
 $\implies a(x^{2} -Sx + P) = 0$

That is, a quadratic whose roots are $\alpha$ and $\beta$, can be written as 
> $x^{2} - (\alpha+\beta)x + \alpha \beta =0$ 

  - A general equation can be written as, 
    $\lambda (x^{2} - (\alpha+\beta)x + \alpha \beta) =0$ 
    Where $\lambda$ is a non-zero constant.

- If a quadratic equation ($=0$) has more than 2 roots, it becomes an identity and the coefficients are all zero.
- If we can observe that the eq. can be written as this, then it may shorten the solution.
  
  ![[Pasted image 20230506080158.png]]

- While calculating an expression of $\alpha, \beta$, it may help to keep in mind that they satisfy the quadratic, hence keep an eye on relative coefficients. 

### Difference of Roots
Difference means subtracting the bigger number from the smaller.
2 difference 3 is 1, while 2 minus 3 is -1. 

It's symbol is '$\sim$'

Difference of Roots = $\alpha \sim \beta = |\alpha - \beta|$ 
> $$\begin{split}
\implies & \left| \left( \frac{-b+\sqrt{D}}{2a} \right) - \left(\frac{-b-\sqrt{D}}{2a} \right) \right|\\
\implies & \left| \left( \frac{2\sqrt{D}}{2a} \right) \right| \\
\implies & \left| \frac{\sqrt{D}}{a} \right|
\end{split}$$

Presence of $D$ in a question can imply the application of difference of roots.