Links: [[07 Tangent and Normal]], [[02.3 Tangent and Normal in Ellipse]], [[03.4 Tangent and Normal in Hyperbola]] 
___
# Tangent and Normal
[[10 General Results for Conics]]

##### Tangent
Equation of tangent to $y^{2} = 4ax$ 

- At $(x_{1},y_{1})$, 
$$yy_{1} = 2a(x + x_{1})$$

- At a point $t$, (replace $y_{1} \to 2at, x_{1} \to at^{2}$)
$$yt = x + at^{2}$$
with slope $m = 1 /t$.
$\\$

- With slope m,
$$y = mx + \frac{ a }{ m }$$


##### Normal
Equation of normal,
- At $(x_{1},y_{1})$ 
  $$y - y_{1} = \frac{ -y_{1} }{ 2a }(x - x_{1})$$
- At point $t$,
	$$y = -tx + 2at + at^{3}$$
	with slope $m = -t$
	$\\$
- With slope m,
  $$y = mx - 2am - am^{3}$$
	From here we can see that **normalcy condition** $c = -2am - am^{3}$

#### Some Results 
If we shift the origin, we have to replace $x \to x - a$ and $y \to y - b$ in the equations of tangent and normal. 
![[Pasted image 20230919090009.png]]

For parabola $x^{2} = 4ay$, 
Tangent at point t i.e. $(2at, at^{2})$,
$$tx = y + at^{2}$$
which is obtained by exchanging x and y in the tangent for $y^{2} = 4ax$

Tangent with slope m,
$$y = mx - am^{2}$$

Normal at point t,
$$x = -ty + 2at + at^{3}$$
Normal with slope m,
$$y = mx + 2a + \frac{ a }{ m^{2} }$$

![[Pasted image 20230919090021.png]]


##### Intersection of tangents and normals
Point of intersection of tangents at $t_{1},t_{2}$, 
$$T:(at_{1}t_{2}, a(t_{1} + t_{2}))$$

Point of intersection of normals at $t_{1},t_{2}$,
$$N:(2a + a(t_{1}^{2} + t_{2}^{2} + t_{1}t_{2}), -at_{1}t_{2}(t_{1} + t_{2}))$$

![[Pasted image 20230919090533.png]]

##### Normal chord
$$
\begin{split}
PQ &: y = -tx + 2at + at^{3} \\
PQ &: 2x - (t + t')y + 2att' = 0 \\
\text{Now}, \\
m_{PQ} &= m_{PQ} \\
-t &= \frac{ 2 }{ t + t' } \\
t' &= -t - \frac{ 2 }{ t }
\end{split}
$$
This is the other point of the normal chord. 

#### Normals from a point
Normal for $y^{2} = 4ax$ is given as
$$y = mx - 2am - am^{3}$$
Now a point $P:(h,k)$ satisfies this,
$$k = mh - 2am - am^{3}$$
$$am^{3} + (2a - h)m + k = 0$$
This is a cubic. Thus it will have at max. 3 real roots. 

$$m_{1} + m_{2} + m_{3} = 0$$
$$m_{1} + m_{2}m_{3} + m_{3}m_{1} = \frac{ 2a - h }{ a }$$
$$m_{1}m_{2}m_{3} = \frac{ -k }{ a }$$

Thus from a point we can draw at max. 3 normals. And min. one normal. 

If the point is inside, we can draw 3 normals. If it is outside then we can draw one. 

Feet of normals A,B,C are called co-normal points. 

![[Pasted image 20230919092630.png]]

If equation of normal is 
$$y = -tx + 2at + at^{3}$$
Then,
$$k = -th + 2at + at^{3}$$
$$at^{3} + (2a - h)t -k = 0$$
this will give the parametric points $t_{A}, t_{B}, t_{C}$.

$$t_{A} + t_{B} + t_{C} = 0$$
From this, 
$$2at_{A} + 2at_{B} + 2at_{C} = 0$$
$$y_{A} + y_{B} + y_{C} = 0$$
i.e. sum of y coordinates of co normal points is zero. 
i.e. centroid of triangle formed by 3 co normal points lie on the axis of the parabola. (for std. parabola it will lie on x axis. )

$$\sum t_{A}t_{B} = \frac{ 2a - h }{ a }$$
Now,
$$
\begin{split}
\sum t_{1}^{2} &= \left( \sum t_{1} \right)^{2} - 2 \sum t_{1}t_{2} \\
&= 0 - \frac{ 2(2a - h) }{ a } \\
&= \frac{ 2(h - 2a) }{ a } 
\end{split}
$$
If all 3 normals are real, then LHS $\geq 0 \implies$ RHS $\geq 0$ and thus $h > 2a$ i.e. $x_{P} > 2a$. 
Note how the reverse is not true i.e. $h > 2a$ does not mean that all 3 are necessarily real. 

##### Normals Intersect on Parabola
If we draw normals and they intersect at the parabola,
$$
\begin{split}
t' &= -t - \frac{2}{t} \\
t^{2} + tt' + 2 &= 0\\
\end{split}
$$
This gives two roots, $t_{1},t_{2}$,
$$
\begin{split}
t_{1} + t_{2} &= -t' \\
t_{1}t_{2} &= 2 
\end{split}
$$
This is the condition that normal drawn at $t_{1},t_{2}$ intersect on the parabola itself.

![[Pasted image 20230919094524.png]]