Links: [[03 T ratio of Sum and Difference of 2 Angles]]
___
# Sum and Difference of Trigonometric ratios
#formula 

### Collectively, to remember
> $$\begin{split}
> \sin C + \sin D &= 2 \sin \left( \frac{C+D}{2} \right) \cdot \cos \left( \frac{C-D}{2} \right) \\\\
> \sin C - \sin D &= 2 \sin \left( \frac{C-D}{2} \right) \cdot \cos \left( \frac{C+D}{2} \right) \\\\ 
> \cos C + \cos D &= 2 \cos \left( \frac{C+D}{2} \right) \cdot \cos \left( \frac{C-D}{2} \right) \\\\
> \cos C - \cos D &= -2 \sin \left( \frac{C+D}{2} \right) \cdot \sin \left( \frac{C-D}{2} \right)
> \end{split}$$

## Proofs
1. $$\sin C + \sin D = 2 \sin \left( \frac{C+D}{2} \right) \cdot \cos \left( \frac{C-D}{2} \right)$$
   
	> Proof:
	> $$\begin{split}
	> \sin (A+B) &= \sin A \cos B + \cos A \sin B \\
	> \sin (A-B) &= \sin A \cos B - \cos A \sin B \\\\
	> \text{Adding them,} &\\
	> \sin (A+B) + \sin (A+B) &= 2 \sin A \cos B \\\\
	> \text{Let,}& \\
	> C &= A + B \\
	> D &= A - B \\
	> \implies & A = \frac{C+D}{2},\ B = \frac{C-D}{2} \\\\
	> \text{Thus, }&\\
	> \sin C + \sin D &= 2 \sin \left(\frac{C+D}{2}\right) \cos \left(\frac{C-D}{2}\right)
	> \end{split}$$

$\\$

2. $$\sin  C - \sin D = 2 \sin \left( \frac{C-D}{2} \right) \cdot \cos \left( \frac{C+D}{2} \right)$$
$\\$

3. $$\cos C + \cos D = 2 \cos \left( \frac{C+D}{2} \right) \cdot \cos \left( \frac{C-D}{2} \right)$$
  	
	> Proof:
	> $$\begin{split}
	> \cos (A+B) &= \cos A \cos B - \sin A \sin B \\
	> \cos (A-B) &= \cos A \cos B + \sin A \sin B \\\\
	> \text{Adding them,} &\\
	> \cos (A+B) + \cos (A+B) &= 2 \cos A \cos B \\\\
	> \text{Let,}& \\
	> C &= A + B \\
	> D &= A - B \\
	> \implies & A = \frac{C+D}{2},\ B = \frac{C-D}{2} \\\\
	> \text{Thus, }&\\
	> \cos C + \cos D &= 2 \cos \left(\frac{C+D}{2}\right) \cos \left(\frac{C-D}{2}\right)
	> \end{split}$$

$\\$

4. $$\cos C - \cos D = -2 \sin \left( \frac{C+D}{2} \right) \cdot \sin \left( \frac{C-D}{2} \right) $$

## Extra results
$$\begin{split}
\sin A \cos B &= \frac{1}{2} (\sin (A+B) + \sin (A-B)) \\\\
\sin A \sin B &= -\frac{1}{2} (\cos (A+B) - \cos (A-B)) \\\\
\cos A \cos B &= \frac{1}{2} (\cos (A+B) + \cos (A-B)) \\\\
\end{split}$$