Links: [[03 T ratio of Sum and Difference of 2 Angles]], [[05 Sum and Difference of T ratios]]
___
# Multiples of Angles
#formula

### Collectively, to remember
> $\sin 2A = 2\sin A \cos A$
> $\phantom{\sin 2A} = (\sin A + \cos A)^{2} - 1$
> $\phantom{\sin 2A} = 1- (\sin A - \cos A)^{2}$
> $\phantom{\sin 2A} = \displaystyle \frac{2 \tan A}{1 + \tan ^{2}A}$
> \
> \
> $\cos 2A = \cos ^{2}A - \sin ^{2}A$ 
> $\phantom{\cos 2A} = 1 - 2\sin ^{2}A$ 
> $\phantom{\cos 2A} = 2\cos ^{2}A - 1$ 
> $\phantom{\cos 2A} = \displaystyle \frac{1 - \tan ^{2}A}{1 + \tan ^{2}A}$ 
> \
> \
> $\tan 2A = \displaystyle \frac{2\tan A}{1-\tan ^{2}A}$
> \
> \
> $\sin 3A = 3 \sin A - 4 \sin ^{3}A$
> $\phantom{\sin 3A} = \sin A(4 \cos ^{2}A-1)$
> \
> \
> $\cos 3A = 4\cos ^{3}A -3\cos A$
> $\phantom{\cos 3A} = \cos A(1- 4\sin ^{2}A)$
> \
> \
> $\tan 3A = \displaystyle \frac{3\tan A - \tan ^{3}A}{1 + 3\tan ^{2}A}$

## Proofs
1. $\sin 2A = 2\sin A \cos A$
$\phantom{\sin 2A} = (\sin A + \cos A)^{2} - 1$
$\phantom{\sin 2A} = 1- (\sin A - \cos A)^{2}$
$\phantom{\sin 2A} = \displaystyle \frac{2 \tan A}{1 + \tan ^{2}A}$

> Proof:
> $$\begin{split}
> \sin 2A &= \sin (A+A) \\
> &= \sin A \cos A + \cos A \sin A \\
> &= 2\sin A \cos A \\
> &= 2 \frac{\sin A}{\cos A}\cos ^{2}A \\
> &= \frac{2\tan A}{\sec ^{2}A} \\
> &= \frac{2\tan A}{1+ \tan ^{2}A} \\
> &= (\sin A + \cos A)^{2} - 1 \\
> &= 1 - (\sin A - \cos A)^{2} 
> \end{split}$$

$\\$

2. $\cos 2A = \cos ^{2}A - \sin ^{2}A$ 
$\phantom{\cos 2A} = 1 - 2\sin ^{2}A$ 
$\phantom{\cos 2A} = 2\cos ^{2}A - 1$ 
$\phantom{\cos 2A} = \displaystyle \frac{1 - \tan ^{2}A}{1 + \tan ^{2}A}$ 

> Proof:
> $$\begin{split}
> \cos 2A &= \cos ^{2}A - \sin ^{2}A \\
> &= \cos ^{2}A - \frac{\sin ^{2}A}{\cos ^{2}A}\cos ^{2}A\\
> &= \cos ^{2}A ( 1 - \tan ^{2}A ) \\
> &= \frac{1 - \tan ^{2}A}{\sec ^{2}A} = \frac{1 - \tan ^{2}A}{1 + \tan ^{2}A}
> \end{split}$$

$\\$

3. $\displaystyle \tan 2A = \frac{2\tan A}{1-\tan ^{2}A}$
Proof: Put $B =A$ in $\tan (A+B)$.

$\\$

4. $\sin 3A = 3 \sin A - 4 \sin ^{3}A$
$\phantom{\sin 3A} = \sin A(4 \cos ^{2}A-1)$
> Proof:
> $$\begin{split}
> \sin 3A &= \sin (A + 2A)\\
> &= \sin A \cos 2A + \cos A \sin 2A\\
> &= \sin A (1 - 2\sin ^{2}A) + \cos A(2\sin A \cos A)\\
> &= \sin A- 2\sin ^{3}A + 2\sin A(1-\sin ^{2}A) \\
> &= 3\sin A - 4 \sin ^{3}A\\
> &= \sin A(3 - 4\sin ^{2}A) \\
> &= \sin A(4\cos^{2}A -1 )
> \end{split}$$

$\\$

5. $\cos 3A = 4\cos ^{3}A -3\cos A$
$\phantom{\cos 3A} = \cos A(1- 4\sin ^{2}A)$
> Proof:
> $$\begin{split}
> \cos 3A &= \cos (A + 2A)\\
> &= \cos A \cos 2A + \sin A \sin 2A\\
> &= \cos A (2\cos ^{2}A - 1) + \sin A(2\sin A \cos A)\\
> &= \cos A- 2\cos ^{3}A + 2\cos A(1-\cos ^{2}A) \\
> &= 4 \cos ^{3}A - 3\cos A\\
> &= \cos A(4\cos ^{2}A - 3) \\
> &= \cos A(1 - 4\sin^{2}A)
> \end{split}$$

$\\$

6. $\tan 3A = \displaystyle \frac{3\tan A - \tan ^{3}A}{1 - 3\tan ^{2}A}$
> Proof:
> $$\begin{split}
> \tan 3A &= \frac{\sin 3A}{\cos 3A} \\
> &= \frac{3 \sin A - 4 \sin ^{3}A}{4\cos ^{3}A - 3 \cos A} \\
> \text{Dividing by } & \cos ^{3}A, \\
> &= \frac{3 \tan A \sec ^{2}A - 4 \tan ^{3}A}{4 - 3\sec ^{2}A} \\
> &= \frac{3\tan A (1 + \sec ^{2}A) - 4\tan ^{3}A}{4 - 3 + 3 \tan ^{2}A}\\
> &= \frac{3\tan A - \tan ^{3}A}{1 - 3\tan ^{2}A}
> \end{split}$$

$\\$

### Some points to remember
1. We can use $\cos 2A$ to convert quadratic terms of $\sin$ and $\cos$ to linear terms.
  
  $$\displaystyle \sin ^{2}A = \frac{1-\cos 2A}{2}$$ $$\displaystyle \cos ^{2}A = \frac{1+\cos 2A}{2}$$
  
2. In the formula $\displaystyle \cos 2A = \frac{1 - \tan ^{2}A}{1 + \tan ^{2}A}$ , $\cos 2A$ and $\tan ^{2}A$ are interchangeable. [[00 Basic Mathematics#Componendo and Divinendo]]
    $$\cos 2A = \frac{1 - \tan ^{2}A}{1 + \tan ^{2}A} \longrightarrow \tan ^{2}A = \frac{1 - \cos 2A}{1 + \cos 2A}$$

3. When angles are doubling with each $\cos$ term, [See this](https://youtu.be/P0XavcgmoOk?list=PL_A4M5IAkMafhPkzpa16mbUDqD8d7bBhL&t=153)
   $$\begin{split}
 \cos (A) \cos (2A) \cos (4A) .....& \cos (2^{n-1}A) \\
&= \frac{\sin A}{\sin A}\cos (A) \cos (2A) \cos (4A) ..... \cos (2^{n-1}A) \\
&= \frac{1}{\sin A} \frac{\sin (2A)}{2} \cos (2A) \cos (4A) ..... \cos (2^{n-1}A) \\
&= \frac{1}{\sin A} \frac{\sin (4A)}{4} \cos (4A) ..... \cos (2^{n-1}A) \\
\text{Thus,} &\\
\cos (A) \cos (2A) ..... \cos (2^{n-1}A) &= \frac{\sin (2^{n}A)}{2^{n}\sin A}
\end{split}$$
![[Cos series double angle.png]]

## Extra Results
- $$\tan A + \cot A = 2 \csc 2A$$
  Use $\sin A \cos A = \displaystyle \frac{ \sin 2A }{ 2 }$ 

- $$\cot A - \tan A = 2 \cot 2A$$
  Use $\sin A \cos A = \displaystyle \frac{ \sin_{2}A }{ 2 }$ and $\cos ^{2}A-\sin ^{2}A = \cos 2A$

- $$\cot A = \cot 2A + \csc 2A$$
  Add the previous 2

- $$\sin (60 - A) \cdot \sin A \cdot \sin (60+A) = \frac{1}{4}\sin 3A$$
  
$$
\begin{split}
\left( \frac{ \sqrt{ 3 } }{ 2 }\cos A - \frac{1}{2}\sin A \right) &\sin A \left( \frac{ \sqrt{ 3 } }{ 2 }\cos A + \frac{ 1 }{ 2 } \cos A \right) \\
\frac{1}{4} &\sin A (3\cos ^{2}A - \sin A) \\
\frac{1}{4}&\sin A(3-4\sin ^{2}A) 
\end{split}
$$

- $$\cos (60 - A) \cdot \cos A \cdot \cos (60+A) = \frac{1}{4}\cos 3A$$

- $$\tan (60 - A) \cdot \tan A \cdot \tan (60+A) = \tan 3A$$

- $$\sin 18 = \frac{\sqrt{5}-1}{4} = \cos 72$$ [See this](https://youtu.be/kReMKFcFF5A?list=PL_A4M5IAkMafhPkzpa16mbUDqD8d7bBhL&t=349)

- $$\cos 36 = \frac{\sqrt{5}+1}{4} = \sin 54$$

- $$\tan \frac{\pi}{8} = \sqrt{2} - 1$$ using $\cos 2A$ and PTR 2.

- $$\cot \frac{\pi}{8} = \sqrt{2} + 1$$
### Sub-Multiples of Angles

1. $$\cos \frac{A}{2} = \pm\sqrt{\frac{1+\cos A}{2}}$$

1. $$\sin \frac{A}{2} = \pm\sqrt{\frac{1-\cos A}{2}}$$

1. $$\tan \frac{A}{2} = \pm\sqrt{\frac{1-\cos A}{1+\cos A}}$$


