Links: [[01 Centre of Mass]]
___
# COM of n discrete particles
Particles are also called *Point masses.*

$$\vec{r}_{com} = \frac{m_{1}\vec{r}_{1} + m_{2}\vec{r}_{2} + m_{3}\vec{r}_{3} + \dots m_{n} \vec{r}_{n}}{m_{1} + m_{2} + m_{3} + \dots m_{n}}$$
$$\vec{r}_{com} = \frac{ \sum m_{1}\vec{r}_{1} }{ \sum m_{1} }$$

We can find the x, y, z coordinate separately also, 
$$x_{com} = \frac{ \sum m_{1}x_{1} }{ \sum m_{1} }$$
$$y_{com} = \frac{ \sum m_{1}y_{1} }{ \sum m_{1} }$$
$$z_{com} = \frac{ \sum m_{1}z_{1} }{ \sum m_{1} }$$


![[Pasted image 20230629132640.png]]


### Sum of Mass Moments about COM

If we sum the mass moments as calculated from the COM instead of the origin, it comes out to be zero. 
$$
\begin{split}
\sum m_{1}\vec{r}_{1c} &= \sum m_{1}(\vec{r}_{1} - \vec{r}_{c}) \\
\\
&= \sum  m_{1}\vec{r}_{1} - \vec{r}_{c}\sum m_{1} \\
\\
&= \sum m_{1}\vec{r}_{1} - M\vec{r}_{c} \\
\\
&= \sum m_{1}\vec{r}_{1} - M \left( \frac{ \sum m_{1}\vec{r}_{1} }{ M } \right) \\
\\
&= \sum m_{1}\vec{r}_{1} - \sum m_{1}\vec{r}_{1} \\
\\
&= \text{Null Vector}
\end{split}
$$

Thus the **summation of mass moments about COM is always zero.** 

## 2 point masses
The COM lies on the line joining the two. 

$$\vec{r}_{com} = \frac{ m_{1}\vec{r}_{1} + m_{2}\vec{r}_{2} }{ m_{1}+m_{2} }$$

If both the particles are on x axis, separated by distance $d$,
$$r_{com} = \left( \frac{ m_{2}d }{ m_{1}+m_{2} }, 0 \right)$$

From the first particle, the COM is at a distance of,
$$x_{1} = \frac{ m_{2}d }{ m_{1}+m_{2} }$$
From the second particle, the COM is at a distance of,
$$x_{1} = \frac{ m_{1}d }{ m_{1}+m_{2} }$$

Their ratio,
$$\frac{ x_{1} }{ x_{2} } = \frac{ m_{2} }{ m_{1} }$$
Thus, the more is the mass, the closer is the COM to it. 

$$x \propto \frac{ 1 }{ m }$$

![[Pasted image 20230629134124.png]]

#### Displacement of one of the Particles
$m_{1}$ is displaced $x_{1}$  left (outwards or away from COM). We need to find by how much and in which direction we need to displace $m_{2}$ such that position of COM does not change. 

We know  that,
$$m_{1}X_{1} = m_{2}X_{2}$$
Thus, if one of the particles is displaced towards left the other will be displaced towards right.

$$m_{1}(X_{1} + x_{1}) = m_{2}(X_{2} + x_{2})$$
$$m_{1}X_{1} + m_{1}x_{1} = m_{2}X_{2} + m_{2}x_{2}$$
$$x_{2} = \frac{ m_{1}x_{1} }{ m_{2} }$$

Thus, 
$$m_{1}x_{1} = m_{2}x_{2}$$
where $x_{1},x_{2}$ are displacements of the particles in opposite directions. 

![[Pasted image 20230629165646.png]]