Links: [[01 Indeterminant form]] 
___
# Evaluation of Limits
1. Find where the given form is determinant or indeterminant.
2. If need be then calculate LHL and RHL separately.
3. Convert given indeterminant form into determinant form. 


### Points to Remember
1. Approaching zero,
	$$
	\begin{split}
	\frac{1}{0^{+}\uparrow} &\to \infty \\ \\
	\frac{1}{0^{-}\uparrow} &\to -\infty
	\end{split}
	$$

2. $\displaystyle \frac{1}{n(n-1)} = \frac{1}{n-1} - \frac{1}{n}$
   $\\$

6. For exponential functions,
	$$
	\begin{split}
	\lim_{ x \to \infty } a^{x} &= 0,\ 0 < a <1 \\
	&= 1,\ a =1 \\
	&= DNE\ (\to \infty),\ a > 1
	\end{split}
	$$


	
3. [[00 Sequence and Series#Sum of some Special Sequences]]
$$
\begin{flalign}
\sum_{r=1}^{n}r &=  \frac{n(n+1)}{2} \\
\sum_{r=1}^{n}r^{2} &=  \frac{n(n+1)(2n+1)}{6} \\
\sum_{r=1}^{n}r^{3} &= \left( \frac{n(n+1)}{2} \right)^{2} 
\end{flalign}
$$

4. [[02 Formula and Expansions]]
$$
\begin{flalign}
\sqrt{x} - \sqrt{y} &= \frac{x-y}{\sqrt{x} + \sqrt{y}} \\
\sqrt{x} - \sqrt{y} &= \frac{x-y}{\sqrt{x} + \sqrt{y}} \\
\sqrt[3]{x} - \sqrt[3]{y} &= \frac{x-y}{x^{\frac{2}{3}} + x^{\frac{1}{3}}y^{\frac{1}{3}} + y^{\frac{2}{3}}} 
\end{flalign}
$$

5. [[08 When angles are in AP]]
   
	$\sin (a) + \sin (a+b) + \sin (a+2b) + sin (a+3b) +......$
	$$
	\begin{flalign}
	\implies \frac{\sin \frac{nb}{2}}{\sin \frac{b}{2}} \cdot \sin \left( \frac{a+a+(n-1)b}{2} \right) &&
	\end{flalign}
	$$

	$\cos (a) + \cos (a+b) + \cos (a+2b) + \cos  (a+3b) +......$
	$$
	\begin{flalign}
	\implies \frac{\sin \frac{nb}{2}}{\sin \frac{b}{2}} \cdot \cos \left( \frac{a + a+(n-1)b}{2} \right) &&
	\end{flalign}
	$$

## [[04 Methods of Evaluation of Limits]]