Links: [[04 Methods of Evaluation of Limits]]
___
# Expansion

If $x \to 0$ then,
[[02 Formula and Expansions#Expansions]]

$$
\begin{split}
e^{ x } &= 1 + \frac{ x }{ 1! } + \frac{ x^{2} }{ 2! } + \frac{ x^{3} }{ 3! } + \dots \\
\\
e^{ -x } &= 1 - \frac{ x }{ 1! } + \frac{ x^{2} }{ 2! } - \frac{ x^{3} }{ 3! } + \dots  \\
\\
a^{ x } &= 1 + \frac{ x\ln a }{ 1! } + \frac{ x^{2}\ln^{2}a }{ 2! } + \frac{ x^{3}\ln^{3}a }{ 3! } + \dots \\
\\
a^{ -x } &= 1 - \frac{ x\ln a }{ 1! } + \frac{ x^{2}\ln^{2}a }{ 2! } - \frac{ x^{3}\ln^{3}a }{ 3! } + \dots \\
\\
\sin x &= x - \frac{ x^{3} }{ 3! } + \frac{ x^{5} }{ 5! } - \frac{ x^{7} }{ 7! } + \dots \\
\\
\cos x &= 1 - \frac{ x^{2} }{ 2! } + \frac{ x^{4} }{ 4! } - \frac{ x^{6} }{ 6! } + \dots \\
\\
\tan x &= x + \frac{ x^{3} }{ 3 } + \frac{ 2x^{5} }{ 15 } + \dots \\
\\
\ln(1 + x) &= x - \frac{ x^{2} }{ 2 } + \frac{ x^{3} }{ 3 } - \frac{ x^{4} }{ 4 } + \dots \\
\\
\ln(1 - x) &= -x - \frac{ x^{2} }{ 2 } - \frac{ x^{3} }{ 3 } - \frac{ x^{4} }{ 4 } - \dots \\
\end{split}
$$

Putting $x = x\ln a$ in the $e^{ x }$ expansion gives $a^{x}$ expansion. 
Taking out the even powers from $e^{ x }$ and putting alternative +, - we get expansion of cos.
Taking out the odd powers from $e^{ x }$ and putting alternative +, - we get expansion of sin. (remember that sin is odd so only odd powers should be there)

In general,
$$f(x) = f(0) + \frac{ f'(0) }{ 1! } + \frac{ f''(0) }{ 2! }x^{2} + \frac{ f'''(0) }{ 3! }x^{3} + \dots$$

This is called Maclaurin series. Which is a special case of Taylor series.

The function can be approximated by this polynomial when $x \to 0$. The more terms we write, the more accurate the approximation. 

If we change the point of approximation from $x \to 0$ to any other point, say a, i.e. $x \to a$, then the $0$s in the expansion are replaced by $a$.

We should expand till 1 more than cancelled in sum form. 
Expansion can only be used when x (or argument) is going to 0. 

Examples,
![[Pasted image 20230807095927.png]]
![[Pasted image 20230807095940.png]]