Links: [[09 Pair of Straight Lines]]
___
# POSL passing through Origin 
The point of intersection of lines is origin. 

Since the lines are passing through centre, the equations of lines will be,
$$L_{1} \equiv y - m_{1}x = 0$$
$$L_{2} \equiv y - m_{2}x = 0$$
Thus their joint equation is given by,
$$
\begin{split}
(y - m_{1}x) (y - m_{2}x) &= 0\\
y^{2} - (m_{1} + m_{2})xy + m_{1}m_{2} x^{2} &= 0
\end{split}
$$

Thus only terms of $y^{2}, xy, x^{2}$ can come in an equation of POSL passing through origin.

Joint equation of POSL passing through origin will be a homogeneous (all terms are of same degree) of degree 2 and vice-versa. 

Any homogeneous equation of degree n will represent n straight lines passing through origin. E.g. HE of degree 3 represents 3 SL passing through origin. 

The equation $x^{2} + by^{2} = 0$ is a HE of degree 2 hence it will represent POSL passing through origin. However, if there are no real factors of this, these POSL are imaginary. 

A general 2 degree HE can be given as,
$$ax^{2} + 2hxy + by^{2} = 0$$
and if it represent $y = m_{1}x$ and $y = m_{2}x$, then, 
$$y^{2} - (m_{1} + m_{2})xy + m_{1}m_{2} x^{2} = 0$$

Comparing coefficients, we get,
$$\frac{ m_{1}m_{2} }{ a } = \frac{ -(m_{1}+m_{2}) }{ 2h } = \frac{ 1 }{ b }$$
Giving,
$$m_{1} + m_{2} = \frac{ -2h }{ b }$$
$$m_{1} m_{2} = \frac{ a }{ b }$$
which are relations between the slopes of the lines. 
- The equation $by^{2} + 2hxy + ax^{2} = 0$ is quadratic in y and the roots are $m_{1}, m_{2}$ (assume as they are not actually) thus using sum and product of roots we get the results above. 

If we divide joint equation of lines by $x^{2}$, then the quadratic equation obtained in variable $\displaystyle\frac{ y }{ x }$ will have roots as the slopes of the lines. 

##### Angle between the lines 
$$ax^{2} + 2hxy + by^{2} = 0$$

The angle between the lines will be,
$$\theta = \tan ^{-1} \left| \frac{ 2\sqrt{ h^{2} - ab } }{ a + b } \right| $$
Which is  the same as in general POSL. 

If $h^{2} = ab$, the lines will be coincident (parallel and passes through origin).
In this case the joint equation will be a perfect square of the type $(a_{1}x + b_{1}y)^{2} = 0$

If $a + b = 0$, the lines will be perpendicular to each other. 

If $h^{2} < ab$ the lines will be imaginary. 
If $h^{2} > ab$ then lines will be distinct real.

#### [[08 Angular Bisector]] 
The angular bisectors are also a pair of straight lines which are passing through origin. 
![[Pasted image 20230713091422.png]]


Now let,
$$L_{1}, L_{2} \equiv ax^{2} + 2hxy + by^{2} = 0$$
$$L_{1} \equiv y = m_{1}x$$
$$L_{2} \equiv y = m_{2}x$$

Then,
$$
\begin{split}
B_{1},B_{2} &\equiv \frac{ L_{1} }{ \sqrt{ a_{1}^{2} + b_{1}s^{2} }  } = \pm \frac{ L_{2} }{ \sqrt{ a_{2}^{2} + b_{2}^{2} } } \\
&= \frac{ y - m_{1}x }{ \sqrt{ 1 + m_{1}^{2} } } = \pm \frac{ y - m_{2}x }{ \sqrt{ 1 + m_{2}^{2} } }
\end{split}
$$
Thus the equations of bisectors will be,
$$B_{1} \equiv \frac{ y - m_{1}x }{ \sqrt{ 1 + m_{1}^{2} } } - \frac{ y - m_{2}x }{ \sqrt{ 1 + m_{2}^{2} } } = 0$$
$$B_{2} \equiv \frac{ y - m_{1}x }{ \sqrt{ 1 + m_{1}^{2} } } + \frac{ y - m_{2}x }{ \sqrt{ 1 + m_{2}^{2} } } = 0$$

For their joint equation, we multiply the above.
$$\frac{ (y - m_{1}x)^{2} }{ 1 + m_{1}^{2} } - \frac{ (y - m_{2}x)^{2} }{ 1 + m_{2}^{2} } = 0$$

Opening square and cross multiplying,
$$y^{2} (m_{2}^{2} - m_{1}^{2}) + x^{2} (m_{1}^{2} - m_{2}^{2}) = 2xy((m_{1} - m_{2}) + m_{2}m_{1}(m_{2} - m_{1}))$$

Dividing by $(m_{1} - m_{2})$,
$$-y^{2}(m_{1} + m_{2}) + x^{2}(m_{1} + m_{2}) = 2xy(1 - m_{1}m_{2})$$
$$(x^{2} + y^{2})(m_{1} + m_{2}) = 2xy(1 - m_{1}m_{2})$$

Putting the values, we get,
$$h(x^{2} - y^{2}) = (a - b)xy$$
$$\frac{ x^{2} - y^{2} }{ a - b } = \frac{ xy }{ h }$$
This is the joint equation of angular bisectors.
